reflection: exposing proper bvs, 5th time is the charm
includes a big refactor of the library

Note: we're still on fully named! This is just an intermediate step.

src/fstar/FStar.Main.fs
@@ -177,6 +177,7 @@ let go _ =
 
 let lazy_chooser k i = match k with
     | FStar.Syntax.Syntax.BadLazy -> failwith "lazy chooser: got a BadLazy"
+    | FStar.Syntax.Syntax.Lazy_bv         -> FStar.Reflection.Embeddings.unfold_lazy_bv          i
     | FStar.Syntax.Syntax.Lazy_binder     -> FStar.Reflection.Embeddings.unfold_lazy_binder      i
     | FStar.Syntax.Syntax.Lazy_fvar       -> FStar.Reflection.Embeddings.unfold_lazy_fvar        i
     | FStar.Syntax.Syntax.Lazy_comp       -> FStar.Reflection.Embeddings.unfold_lazy_comp        i
