ulib/FStar.Reflection.Data.fst
@@ -28,17 +28,25 @@ type aqualv =
 type argv = term * aqualv
 
 noeq
+type bv_view = {
+    ppname : string;
+    index : int;
+    sort : typ;
+}
+
+noeq
 type term_view =
-  | Tv_Var    : binder -> term_view
+  | Tv_Var    : bv -> term_view
+  | Tv_BVar   : bv -> term_view
   | Tv_FVar   : fv -> term_view
   | Tv_App    : term -> argv -> term_view
   | Tv_Abs    : binder -> term -> term_view
   | Tv_Arrow  : binder -> comp -> term_view
   | Tv_Type   : unit -> term_view
-  | Tv_Refine : binder -> term -> term_view
+  | Tv_Refine : bv -> term -> term_view
   | Tv_Const  : vconst -> term_view
   | Tv_Uvar   : int -> typ -> term_view
-  | Tv_Let    : bool -> binder -> term -> term -> term_view
+  | Tv_Let    : bool -> bv -> term -> term -> term_view
   | Tv_Match  : term -> list branch -> term_view
   | Tv_Unknown : term_view // Baked in "None"
 
@@ -77,3 +85,54 @@ type sigelt_view =
   | Unk
 
 type decls = list sigelt
+
+let rec forall_list (p:'a -> Type) (l:list 'a) : Type =
+    match l with
+    | [] -> True
+    | x::xs -> p x /\ forall_list p xs
+
+(* Comparison of a term_view to term. Allows to recurse while changing the view *)
+val smaller : term_view -> term -> Type0
+let smaller tv t =
+    match tv with
+    | Tv_App l r ->
+        l << t /\ r << t /\ fst r << t
+
+    | Tv_Abs b t'
+    | Tv_Arrow b t' ->
+        b << t /\ t' << t
+
+    | Tv_Refine b t' ->
+        bv << t /\ t' << t
+
+    | Tv_Let r bv t1 t2 ->
+        bv << t /\ t1 << t /\ t2 << t
+
+    | Tv_Match t1 brs ->
+        t1 << t /\ (forall_list (fun (b, t') -> t' << t) brs)
+
+    | Tv_Type _
+    | Tv_Const _
+    | Tv_Unknown
+    | Tv_Var _
+    | Tv_BVar _
+    | Tv_Uvar _ _
+    | Tv_FVar _ -> True
+
+val smaller_comp : comp_view -> comp -> Type0
+let smaller_comp cv c =
+    match cv with
+    | C_Total t ->
+        t << c
+    | C_Lemma pre post ->
+        pre << c /\ post << c
+    | C_Unknown ->
+        True
+
+val smaller_bv : bv_view -> bv -> Type0
+let smaller_bv bvv bv =
+    bvv.sort << bv
+
+val smaller_binder : binder -> (bv * aqualv) -> Type0
+let smaller_binder b (bv, _) =
+    bv << b
